Extraction: add extension passes as for Krml
This will be used by Pulse. Ideally, again, this would be a more
well-defined reflection API.

src/extraction/FStarC.Extraction.ML.Term.fsti
@@ -25,5 +25,12 @@ val normalize_for_extraction (env:uenv) (e:term) : term
 val is_arity: uenv -> term -> bool
 val ind_discriminator_body : env:uenv -> discName:lident -> constrName:lident -> mlmodule1
 val term_as_mlty: uenv -> term -> mlty
+
+exception NotSupportedByExtension
+let translate_typ_t = g:uenv -> t:term -> mlty
+val register_pre_translate_typ (f : translate_typ_t) : unit
+let translate_t = g:uenv -> t:term -> mlexpr & e_tag & mlty
+val register_pre_translate (f : translate_t) : unit
+
 val term_as_mlexpr: uenv -> term -> mlexpr & e_tag & mlty
 val extract_lb_iface : uenv -> letbindings -> uenv & list (fv & exp_binding)
